lib/steel/pulse/Pulse.Typing.fst
@@ -412,7 +412,6 @@ let comp_admit (c:ctag) (s:st_comp) : comp =
 noeq
 type my_erased (a:Type) = | E of a
 
-
 let typing (g:env) (e:term) (t:term) =
     RT.tot_typing (elab_env g) (elab_term e) (elab_term t)
 
@@ -443,8 +442,8 @@ type st_equiv : env -> comp -> comp -> Type =
       tot_typing g (comp_pre c1) tm_vprop ->
       tot_typing g (comp_res c1) (tm_type (comp_u c1)) ->
       tot_typing (push_binding g x ppname_default (comp_res c1)) (open_term (comp_post c1) x) tm_vprop ->
-      vprop_equiv g (comp_pre c1) (comp_pre c2) ->
-      vprop_equiv (push_binding g x ppname_default (comp_res c1))
+      equiv_pre: vprop_equiv g (comp_pre c1) (comp_pre c2) ->
+      equiv_post: vprop_equiv (push_binding g x ppname_default (comp_res c1))
                   (open_term (comp_post c1) x)
                   (open_term (comp_post c2) x) ->      
       st_equiv g c1 c2
